Make some ltac and clean up Fix _CoqProject

Aexp.v
@@ -5,8 +5,9 @@ From Rela Require Import Loc.
 
 Inductive aexp : Type :=
   | ANum (n : nat)
-  | AId (x : Loc.t)
-  | AP (x: Loc.t)
+  | ARef (x : Loc.t)
+  | AId (x: Loc.t)
+  | Aadd (x: Loc.t)
   | APlus (a1 a2 : aexp)
   | AMinus (a1 a2 : aexp)
   | AMult (a1 a2 : aexp).
@@ -16,8 +17,9 @@ Inductive aexp : Type :=
 Fixpoint aeval (st : sigma) (a : aexp) : nat :=
   match a with
   | ANum n => n
-  | AId x => st (x)
-  | AP x => x
+  | AId x => st x
+  | ARef x => st (st x)
+  | Aadd x => x
   | APlus a1 a2 => (aeval st a1) + (aeval st a2)
   | AMinus a1 a2 => (aeval st a1) - (aeval st a2)
   | AMult a1 a2 => (aeval st a1) * (aeval st a2)
@@ -31,14 +33,16 @@ Declare Custom Entry aexp.
 
 Module AexpNotations.
 
-Coercion AP : Loc.t >-> aexp.
+Coercion AId : Loc.t >-> aexp.
 Coercion ANum : nat >-> aexp.
 
 Notation "[? e ?]" := (e) (e custom aexp at level 0) : aexp_scope.
 Notation "x" := x (in custom aexp at level 0, x constr at level 0) : aexp_scope.
 Notation "( x )" := x (in custom aexp,
                        x custom aexp at level 2) : aexp_scope.
-Notation "'°' x" := (AId x) (in custom aexp at level 30,
+Notation "'°' x" := (ARef x) (in custom aexp at level 30,
+                         x custom aexp ) : aexp_scope.
+Notation "'&' x" := (Aadd x) (in custom aexp at level 30,
                          x custom aexp ) : aexp_scope.
 Notation "x + y" := (APlus x y) (in custom aexp at level 50,
                                  x custom aexp,
