Examples.v
@@ -4,6 +4,7 @@ From Rela Require Import Aexp.
 From Rela Require Import Bexp.
 From Rela Require Import Com.
 From Rela Require Import Vcg.
+From Rela Require Vcg_Opt.
 From Rela Require Import Hoare_Triple.
 From Rela Require Import Correct.
 From Rela Require Import Rela.
@@ -11,19 +12,17 @@ Import Vcg.Why3_Set.
 Import Vcg.Assn_b.
 From Coq Require Import Lists.List.
 Import ListNotations.
-Require Import Program.
-Require Import Eqdep_dec.
+From Coq Require Import Program.
+From Coq Require Import Eqdep_dec.
 From Coq Require Import Lia.
 
 (** Example of arithmetic expression **)
 
 Import AexpNotations.
 
-Definition example_aexp : aexp := [? EAX + 2 + (°EAX * 2) ?].
-
 Example aexp1 :
 forall st : sigma,
-    aeval (EAX !-> 5 ; st) example_aexp = 13.
+    aeval (EAX !-> 1 ; st) [? (EAX + °EAX + &EAX) * 2 ?] = 6.
 Proof.
 reflexivity.
 Qed.
@@ -32,13 +31,9 @@ Qed.
 
 Import BexpNotations.
 
-Definition example_bexp : bexp := [! true && ~ °EAX <= 4 !].
-
-Print Visibility.
-
 Example bexp1 :
 forall st : sigma,
-    beval (EAX !-> 5 ; st) example_bexp = true.
+    beval (EAX !-> 5 ; st) [! true && ~ EAX <= 4 !] = true.
 Proof.
 reflexivity.
 Qed.
@@ -47,7 +42,7 @@ Qed.
 
 Import ComNotations.
 
-Definition plus2 : com := <[ EAX := °EAX + 2 ]>.
+Definition plus2 : com := <[ EAX := EAX + 2 ]>.
 
 Example ecom3 :
 forall (s : sigma),
@@ -55,17 +50,14 @@ forall (s : sigma),
 Proof.
 intros.
 unfold plus2.
-apply E_Ass. reflexivity. reflexivity.
+apply E_Ass. reflexivity.
 Qed.
-
-Definition assert2 : com := <[ assert (fun s => s EAX = 2) ]>.
 
 Example ecom4 :
 forall (s : sigma),
-  ceval assert2 (EAX !-> 2 ; s) Psi.empty_psi (EAX !-> 2 ; s).
+  ceval <[ assert (fun s => s EAX = 2) ]> (EAX !-> 2 ; s) Psi.empty_psi (EAX !-> 2 ; s).
 Proof.
 intros.
-unfold assert2.
 apply E_Assert. apply get_sigma_same.
 Qed.
 
@@ -87,7 +79,7 @@ apply recursion_hoare_triple with Phi.empty_phi.
     reflexivity.
 Qed.
 
-Definition plus3 : com := <[ EAX := °EAX + 2; EAX := °EAX + 2 ]>.
+Definition plus3 : com := <[ EAX := EAX + 2; EAX := EAX + 2 ]>.
 
 Example Haore2 : hoare_triple (fun m => m EAX = 1) (fun m' => m' EAX = 5) plus3 Psi.empty_psi.
 Proof.
@@ -105,7 +97,7 @@ apply recursion_hoare_triple with Phi.empty_phi.
     reflexivity.
 Qed.
 
-Definition if2 : com := <[ if °EAX = 4 then { plus2 } else { plus2 } end ]>.
+Definition if2 : com := <[ if EAX = 4 then { plus2 } else { plus2 } end ]>.
 
 Example Hoare3 : hoare_triple (fun m => m EAX = 1) (fun m' => m' EAX = 3) if2 Psi.empty_psi .
 Proof.
@@ -132,8 +124,8 @@ apply recursion_hoare_triple with Phi.empty_phi.
          reflexivity.
 Qed.
 
-Definition if3 : com := <[ EAX := °EAX + 2 ;
-                          if °EAX = 4 then { plus2 } else { plus2 } end;
+Definition if3 : com := <[ EAX := EAX + 2 ;
+                          if EAX = 4 then { plus2 } else { plus2 } end;
                           { plus2 } ]>.
 
 Example Hoare4 : hoare_triple (fun m => m EAX = 1) (fun m' => m' EAX = 7) if3 Psi.empty_psi.
@@ -183,7 +175,7 @@ apply recursion_hoare_triple with Phi.empty_phi.
   + simpl; intros. auto.
 Qed.
 
-Definition if4 : com := <[ if °EAX = 2 then assert (fun m => m EAX = 2) else skip end ]>.
+Definition if4 : com := <[ if EAX = 2 then assert (fun m => m EAX = 2) else skip end ]>.
 
 Example Hoare7 : hoare_triple (fun m => m EAX = 2) (fun m' => m' EAX = 2) if4 Psi.empty_psi.
 Proof.
@@ -210,98 +202,110 @@ apply recursion_hoare_triple with Phi.empty_phi.
          assumption.
 Qed.
 
+(** Some ltac to mechanize the extraction of proof obligation from the list construct **)
+
+Ltac ltc3 hy :=
+  inversion hy as [H1];
+  symmetry in H1;
+  apply length_zero_iff_nil in H1;
+  subst.
+
+Ltac ltc2 phi hy :=
+         destruct (mk_rtc'_def _ _ phi _ _ hy) as (hyr & HYP);
+         rewrite HYP;
+         clear HYP hy;
+         rename hyr into hy.
+
+Ltac ltc7 phi hy H:= 
+  ltc2 phi hy;
+  split;[clear hy; inversion H; clear H; apply Vcg_Opt.tc'_same 
+        | first [ ltc7 phi hy H| simpl;auto]].
+
+Ltac ltc1 phi hy ml H :=
+         destruct ml;
+         [ discriminate hy
+         | first [ltc3 hy; ltc7 phi hy H| ltc1 phi hy ml H]
+         ].
+
+Ltac ltc6 phi hy :=
+       destruct (mk_rtc_def _ _ phi _ _ hy) as (hyr & HYP);
+       rewrite HYP;
+       clear HYP hy;
+       rename hyr into hy.
+
+Ltac ltc5 phi hy :=
+    intro;
+    intros H1;
+    tryif ltc6 Phi.empty_phi hy;
+          eapply consequence_tc_suite;
+          [ clear H1; ltc5 phi hy | apply Vcg_Opt.tc_same; apply H1]
+    then auto
+    else simpl; apply H1.
+
+Ltac ltc4 ml hy phi:=
+         destruct ml;
+         [ discriminate hy
+         | first [ltc3 hy;
+                  ltc6 Phi.empty_phi hy;
+                  eapply consequence_tc_suite;[ ltc5 phi hy | apply Vcg_Opt.tc_same]
+                 | ltc4 ml hy phi]
+          ].
+
+Ltac ltc0 phi := apply rcorrect with phi; 
+                 [ 
+                 | intros ml hy H;
+                   ltc1 phi hy ml H
+                 | intros ml hy H;
+                   ltc4 ml hy phi;
+                   clear hy;
+                   inversion H;
+                   clear H
+                ].
 
 (** Examples of proofs of Relational Properties **)
 
-Definition rela_pre2 (l : list Sigma.sigma) : Prop :=
+Definition rela_pre3 (l : list Sigma.sigma) : Prop :=
   match l with
-  | (m1 :: m2 :: []) => m1 EAX = m2 EAX
+  | (m1 :: m2 :: m3 :: []) => m1 EAX = m2 EAX /\ m2 EAX = m3 EAX
   | _ => False
   end.
 
-Definition rela_post2 (l : list Sigma.sigma) : Prop :=
+Definition rela_post3 (l : list Sigma.sigma) : Prop :=
   match l with
-  | (m1 :: m2 :: []) => m1 EAX = m2 EAX
+  | (m1 :: m2 :: m3 :: []) => m1 EAX = m2 EAX /\ m2 EAX = m3 EAX
   | _ => False
   end.
 
-Example Relation2 : relational_prop rela_pre2 rela_post2 (plus2 :: plus2 :: []) Psi.empty_psi.
+Example Relation3 : relational_prop rela_pre3 rela_post3 
+                    (plus2 :: plus2 :: plus2 :: []) Psi.empty_psi.
 Proof.
-apply rcorrect  with Phi.empty_phi.
-(* Verification of proofs proof obligation for procedure *)
+ltc0 Phi.empty_phi.
+(* Verification of proofs obligation for procedure *)
 + apply tc_p_empty_psi.
-(* Extracting auxiliary proofs proof obligation *)
-+ intros.
-  destruct ml.
-  * discriminate hy.
-  * destruct (mk_rtc'_def plus2 (plus2::[]) Phi.empty_phi s ml hy) as (hyr & HYP).
-    rewrite HYP.
-    split.
-    - simpl. auto.
-    - destruct ml.
-      ++ discriminate hyr.
-      ++ destruct (mk_rtc'_def plus2 [] Phi.empty_phi s0 ml hyr) as (hyr2 & HYP2).
-        rewrite HYP2.
-        split.
-        ** simpl. auto.
-        ** inversion hyr2.
-          symmetry in H1.
-          apply length_zero_iff_nil in H1.
-          subst.
-          simpl.
-          (* Verification of auxiliary proofs proof obligation *)
-           auto.
-(* Extracting main proof obligation *)
-+ intros.
-  destruct ml.
-  * discriminate hy.
-  * destruct (mk_rtc_def rela_post2 plus2 (plus2::[]) Phi.empty_phi s ml hy) as (hyr & HYP).
-    rewrite HYP.
-    destruct ml.
-    - discriminate hyr.
-    - assert (H1 : length ([] : list com) = length ml).
-      { inversion hyr. reflexivity. }
-      eapply Vcg.consequence_tc_suite.
-      ++ intros.
-         destruct (mk_rtc_def (fun l : list sigma => rela_post2 (s1 :: l)) plus2 [] Phi.empty_phi s0 ml hyr) as (hyr2 & HYP2).
-         rewrite HYP2.
-         replace hyr2 with H1.
-         ** apply (Vcg.consequence_tc_suite _ _ _ (fun m' => s1 EAX = m' EAX)).
-            -- intros.
-               inversion hyr2.
-               symmetry in H4.
-               apply length_zero_iff_nil in H4.
-               subst.
-               simpl.
-               apply H2.
-           -- apply H0.
-         ** apply eq_proofs_unicity.
-            intros.
-            lia.
-      ++ (* Extracting relational precondition *) 
-         inversion H1.
-         symmetry in H2.
-         apply length_zero_iff_nil in H2.
-         subst.
-         simpl in H.
-         (* Proof on main proof obligation *)
-         simpl.
-         intros.
-         rewrite H2.
-         rewrite H0.
-         rewrite H.
-         apply Why3_Set.set'def.
-         reflexivity.
+(* Verification of auxilliary proof obligation *)
++ simpl. auto.
++ simpl. auto.
++ simpl. auto.
+(* Main proof obligation *)
++ simpl.
+  intros.
+  rewrite H3.
+  rewrite H.
+  rewrite H2.
+  rewrite H0.
+  rewrite H1.
+  split.
+  all: try apply Why3_Set.set'def;reflexivity.
 Qed.
 
 Definition X1 : Loc.t:= 1.
 Definition X2 : Loc.t:= 2.
 Definition ret : Loc.t := 3.
 
-Definition comp: com := <[ if °X1 <= °X2 && ~ °X1 = °X2 then
+Definition comp: com := <[ if X1 <= X2 && ~ X1 = X2 then
                                  ret := 0
                               else
-                                 if °X2 <= °X1 && ~ °X1 = °X2  then
+                                 if X2 <= X1 && ~ X1 = X2  then
                                    ret := 2
                                  else ret := 1
                                  end
@@ -323,111 +327,38 @@ Example Relation_comp : relational_prop
                             rela_pre_comp rela_post_comp
                             (comp :: comp :: []) Psi.empty_psi.
 Proof.
-apply rcorrect  with Phi.empty_phi.
-(* Verification of proofs proof obligation for procedure *)
+ltc0 Phi.empty_phi.
+(* Verification of auxiliary proofs proof obligation for procedure*)
 + apply tc_p_empty_psi.
-(* Extracting auxiliary proofs proof obligation *)
-+ intros.
-  destruct ml.
-  * discriminate hy.
-  * destruct (mk_rtc'_def comp (comp::[]) Phi.empty_phi s ml hy) as (hyr & HYP).
-    rewrite HYP.
-    split.
-    - simpl. auto. (* Verification of auxiliary proofs proof obligation for function 1*)
-
-    - destruct ml.
-      ++ discriminate hyr.
-      ++ destruct (mk_rtc'_def comp [] Phi.empty_phi s0 ml hyr) as (hyr2 & HYP2).
-        rewrite HYP2.
-        split.
-        ** simpl. auto. (* Verification of auxiliary proofs
-                           proof obligation for function 1*)
-
-        ** inversion hyr2.
-          symmetry in H1.
-          apply length_zero_iff_nil in H1.
-          subst.
-          simpl.  auto.
-(* Extracting main proof obligation *)
-+ intros.
-  destruct ml.
-  * discriminate hy.
-  * destruct
-      (mk_rtc_def rela_post_comp comp
-      (comp::[]) Phi.empty_phi s ml hy) as (hyr & HYP).
-    rewrite HYP.
-    destruct ml.
-    - discriminate hyr.
-    - assert (H1 : length ([] : list com) = length ml).
-      { inversion hyr. reflexivity. }
-      eapply Vcg.consequence_tc_suite.
-      ++ intros.
-         destruct
-           (mk_rtc_def (fun l : list sigma => rela_post_comp (s1 :: l))
-            comp [] Phi.empty_phi s0 ml hyr) as (hyr2 & HYP2).
-         rewrite HYP2.
-         replace hyr2 with H1.
-         ** apply (Vcg.consequence_tc_suite _ _ _ (fun m' => s1 ret + m' ret = 2)).
-            -- intros.
-               inversion hyr2.
-               symmetry in H4.
-               apply length_zero_iff_nil in H4.
-               subst.
-               simpl.
-               apply H2.
-           -- apply Vcg_Opt.tc_same. apply H0.
-         ** apply eq_proofs_unicity.
-            intros.
-            lia.
-      ++ (* Extracting relational precondition *)
-         inversion H1.
-         symmetry in H2.
-         apply length_zero_iff_nil in H2.
-         subst.
-         simpl in H.
-         (* Proof on main proof obligation *)
-         apply Vcg_Opt.tc_same.
-         simpl.
-         intros.
-         destruct H.
-         destruct H0.
-         -- destruct H2.
-            ** subst.
-            assert(H6: False).
-            { lia. }
-            contradiction H6.
-            ** destruct H5.
-              +++ subst.
-                  rewrite (set''def _ _ _ 0).
-                  rewrite (set''def _ _ _ 2).
-                  all: try reflexivity.
-              +++ subst.
-                  assert(H6: False).
-                  { lia. }
-                  contradiction H6.
-          -- destruct H2.
-            ** destruct H4.
-              +++ subst.
-                  rewrite (set''def _ _ _ 2).
-                  rewrite (set''def _ _ _ 0).
-                  all: try reflexivity.
-              +++ subst.
-                  assert(H6: False).
-                  { lia. }
-                  contradiction H6.
-            ** destruct H4.
-              +++  subst.
-                   assert(H6: False).
-                   { lia. }
-                   contradiction H6.
-              +++ destruct H5.
-                  *** subst.
-                      subst.
-                      assert(H6: False).
-                      { lia. }
-                      contradiction H6.
-                  *** subst.
-                      rewrite (set''def _ _ _ 1).
-                      rewrite (set''def _ _ _ 1).
-                      all: try reflexivity.
+(* Verification of auxilliary proof obligation *)
++ simpl. auto.
++ simpl. auto.
+(* Main proof obligation *)
++ simpl.
+  intros.
+  destruct H.
+  destruct H0.
+  -- destruct H2.
+     ** subst. lia.
+     ** destruct H2.
+        +++ subst.
+            rewrite (set''def _ _ _ 0).
+            rewrite (set''def _ _ _ 2).
+            all: try reflexivity.
+        +++ subst. lia.
+  -- destruct H2.
+     ** destruct H3.
+        +++ subst.
+            rewrite (set''def _ _ _ 2).
+            rewrite (set''def _ _ _ 0).
+            all: try reflexivity.
+        +++ subst. lia.
+     ** destruct H4.
+        +++  subst. lia.
+        +++ destruct H3.
+           *** subst. lia.
+           *** subst.
+               rewrite (set''def _ _ _ 1).
+               rewrite (set''def _ _ _ 1).
+               all: try reflexivity.
 Qed.
